theories/typing.v
@@ -1,9 +1,21 @@
 From iris.heap_lang Require Export lang.
 Require Import FunctionalExtensionality.
 
+
+Class Involutive {T} (f : T → T) :=
+  involutive : ∀ t : T, t = f (f t).
+
 Inductive side : Set :=
 | Left
 | Right.
+
+Instance side_inhabited : Inhabited side := populate Left.
+
+Definition dual_side (s : side) : side :=
+  match s with Left => Right | Right => Left end.
+
+Instance dual_side_involutive : Involutive dual_side.
+Proof. intros s; destruct s; eauto. Qed.
 
 Inductive stype :=
 | TEnd
@@ -18,9 +30,6 @@ Fixpoint dual_stype (st :stype) :=
   | TSend P st => TRecv P (λ v, dual_stype (st v))
   | TRecv P st => TSend P (λ v, dual_stype (st v))
   end.
-
-Class Involutive {T} (f : T → T) :=
-  involutive : ∀ t : T, t = f (f t).
 
 Instance dual_stype_involutive : Involutive dual_stype.
 Proof.
